

Product-of-sums form and maxterms

Product-of-sums form

A **sum term** is an ORing of (one or more) variables

a $(a + b')$ $(a + b' + c')$

$a' + cd$



sum term must only have OR, **not AND**

product-of-sums (POS) form consists solely of
an ANDing of sum terms:

a $(a + b')$ $(a' + c)(b + d)$ $(a + b' + c)(a + b)$

$a' + cd$



$(ab') + (a'c)$

maxterm and Product-of-maxterms form

A **maxterm** is a sum term that has all of the function variables exactly once in either true or complemented form.

For a function of three variables: a, b, and c

$$(a' + b' + c)$$

$$(a' + b + c')$$

$$(a' + b' + c')$$

$(a' + b') \rightarrow c$ representation is missing

$(a' + b' + bc) \rightarrow$ not a sum term



Product-of-maxterms form is a **canonical** form of a Boolean equation where the right-side expression is a product-of-sum with each sum consisting only of maxterms.

For a function of three variables: a, b, and c

$$y = (a' + b' + c')$$

Product-of-maxterms

maxterm and Product-of-maxterms form

A **maxterm** is a sum term that has all of the function variables exactly once in either true or complemented form.

For a function of three variables: a, b, and c

$$(a' + b' + c)$$

$$(a' + b + c')$$

$$(a' + b' + c')$$

$(a' + b') \rightarrow c$ representation is missing

$(a' + b' + bc) \rightarrow$ not a sum term



Product-of-maxterms form is a **canonical** form of a Boolean equation where the right-side expression is a product-of-sum with each sum consisting only of maxterms.

For a function of three variables: a, b, and c

$$y = (a + b + c)(a' + b' + c')$$

Product-of-maxterms

maxterm and Product-of-maxterms form

A **maxterm** is a sum term that has all of the function variables exactly once in either true or complemented form.

For a function of three variables: a, b, and c

$$(a' + b' + c)$$

$$(a' + b + c')$$

$$(a' + b' + c')$$

$(a' + b') \rightarrow c$ representation is missing

$(a' + b' + bc) \rightarrow$ not a sum term



Product-of-maxterms form is a **canonical** form of a Boolean equation where the right-side expression is a product-of-sum with each sum consisting only of maxterms.

For a function of three variables: a, b, and c

$$y = (a' + b)(a' + b' + c')$$



Product-of-maxterms

Truth Tables → Product-of-maxterms form

		inputs			output
		a	b	f	
M_0	$a + b$	0	0	0	←
M_1	$a + b'$	0	1	1	
M_2	$a' + b$	1	0	1	
M_3	$a' + b'$	1	1	0	←

→ $f(a,b) = (a+b)(a'+b')$

Each row of the truth table corresponds to a *maxterm*, denoted by M_x

Any input that has value of **0** → variable is in the true from for our *maxterm*.

Any input that has value of **1** → variable is in the complemented from for our *maxterm*.

For each row where output is 0:

convert truth table to a product-of-maxterms form by ANDing the *maxterms*

converting from product-of-sums to sum-of-products

Converting from POS to SOP:

$$y = (a + b)(a' + b')$$

Product-of-sums form

$$y = a(a' + b') + b(a' + b')$$

Distributive

$$y = aa' + ab' + a'b + bb'$$

Distributive

$$y = 0 + ab' + a'b + 0$$

Complement (AND)

$$y = ab' + a'b$$

Sum-of-products form

				<i>Minterms</i>		<i>Maxterms</i>
<i>X</i>	<i>Y</i>	<i>Z</i>		<i>Product Terms</i>		<i>Sum Terms</i>
0	0	0		$m_0 = \overline{X} \cdot \overline{Y} \cdot \overline{Z} = \min(\overline{X}, \overline{Y}, \overline{Z})$		$M_0 = X + Y + Z = \max(X, Y, Z)$
0	0	1		$m_1 = \overline{X} \cdot \overline{Y} \cdot Z = \min(\overline{X}, \overline{Y}, Z)$		$M_1 = X + Y + \overline{Z} = \max(X, Y, \overline{Z})$
0	1	0		$m_2 = \overline{X} \cdot Y \cdot \overline{Z} = \min(\overline{X}, Y, \overline{Z})$		$M_2 = X + \overline{Y} + Z = \max(X, \overline{Y}, Z)$
0	1	1		$m_3 = \overline{X} \cdot Y \cdot Z = \min(\overline{X}, Y, Z)$		$M_3 = X + \overline{Y} + \overline{Z} = \max(X, \overline{Y}, \overline{Z})$
1	0	0		$m_4 = X \cdot \overline{Y} \cdot \overline{Z} = \min(X, \overline{Y}, \overline{Z})$		$M_4 = \overline{X} + Y + Z = \max(\overline{X}, Y, Z)$
1	0	1		$m_5 = X \cdot \overline{Y} \cdot Z = \min(X, \overline{Y}, Z)$		$M_5 = \overline{X} + Y + \overline{Z} = \max(\overline{X}, Y, \overline{Z})$
1	1	0		$m_6 = X \cdot Y \cdot \overline{Z} = \min(X, Y, \overline{Z})$		$M_6 = \overline{X} + \overline{Y} + Z = \max(\overline{X}, \overline{Y}, Z)$
1	1	1		$m_7 = X \cdot Y \cdot Z = \min(X, Y, Z)$		$M_7 = \overline{X} + \overline{Y} + \overline{Z} = \max(\overline{X}, \overline{Y}, \overline{Z})$